src/Init/Data/Iterators.lean
@@ -3,5 +3,10 @@ Copyright (c) 2025 Lean FRO, LLC. All rights reserved.
 Released under Apache 2.0 license as described in the file LICENSE.
 Authors: Paul Reichert
 -/
+module
+
 prelude
-import Std.Data.Iterators.Internal.Termination
+import Init.Data.Iterators.Basic
+import Init.Data.Iterators.PostconditionMonad
+import Init.Data.Iterators.Consumers
+import Init.Data.Iterators.Lemmas
