src/Init/Data/Iterators/Internal.lean
@@ -3,7 +3,8 @@ Copyright (c) 2025 Lean FRO, LLC. All rights reserved.
 Released under Apache 2.0 license as described in the file LICENSE.
 Authors: Paul Reichert
 -/
+module
+
 prelude
-import Std.Data.Iterators.Consumers.Monadic.Collect
-import Std.Data.Iterators.Consumers.Monadic.Loop
-import Std.Data.Iterators.Consumers.Monadic.Partial
+import Init.Data.Iterators.Internal.LawfulMonadLiftFunction
+import Init.Data.Iterators.Internal.Termination
