src/Std/Data/Iterators/Combinators/Monadic/DropWhile.lean
@@ -6,11 +6,11 @@ Authors: Paul Reichert
 prelude
 import Init.Data.Nat.Lemmas
 import Init.RCases
-import Std.Data.Iterators.Basic
-import Std.Data.Iterators.Consumers.Monadic.Collect
-import Std.Data.Iterators.Consumers.Monadic.Loop
-import Std.Data.Iterators.Internal.Termination
-import Std.Data.Iterators.PostConditionMonad
+import Init.Data.Iterators.Basic
+import Init.Data.Iterators.Consumers.Monadic.Collect
+import Init.Data.Iterators.Consumers.Monadic.Loop
+import Init.Data.Iterators.Internal.Termination
+import Init.Data.Iterators.PostconditionMonad
 
 /-!
 # Monadic `dropWhile` iterator combinator
@@ -278,7 +278,7 @@ instance DropWhile.instIteratorCollectPartial [Monad m] [Monad n] [Iterator α m
   .defaultImplementation
 
 instance DropWhile.instIteratorLoop [Monad m] [Monad n] [Iterator α m β] :
-    IteratorLoop α m n :=
+    IteratorLoop (DropWhile α m β P) m n :=
   .defaultImplementation
 
 instance DropWhile.instIteratorForPartial [Monad m] [Monad n] [Iterator α m β]
