src/Std/Data/Iterators/Combinators/Monadic/FilterMap.lean
@@ -4,11 +4,11 @@ Released under Apache 2.0 license as described in the file LICENSE.
 Authors: Paul Reichert
 -/
 prelude
-import Std.Data.Iterators.Basic
-import Std.Data.Iterators.Consumers.Collect
-import Std.Data.Iterators.Consumers.Loop
-import Std.Data.Iterators.PostConditionMonad
-import Std.Data.Iterators.Internal.Termination
+import Init.Data.Iterators.Basic
+import Init.Data.Iterators.Consumers.Collect
+import Init.Data.Iterators.Consumers.Loop
+import Init.Data.Iterators.PostconditionMonad
+import Init.Data.Iterators.Internal.Termination
 
 /-!
 
